projectVampire/dafny/blood.dfy
@@ -54,10 +54,10 @@ class Blood{
         rh := rhesus;
     }
 
-    method get_state() returns (bl_state:blood_state)
-    ensures bl_state == state
+    function method get_state(): blood_state
+	reads this
     {
-        bl_state := state;
+        state
     }
 
     constructor (secondsin:int)
@@ -71,7 +71,7 @@ class Blood{
         state := unverified;
     }
 
-    method verify_blood(curr_time:int,accepted:bool,determined_type:Blood_types,rhesus_in:bool)
+    method verify_blood(curr_time:int,accepted:bool,determined_type:Blood_types,rhesus_in:bool) returns (success:bool)
     modifies this;
     requires state==unverified
     requires Valid()
@@ -79,56 +79,79 @@ class Blood{
     ensures blood_type==determined_type
     ensures rhesus == rhesus_in
     ensures Valid()
+	ensures if success then state==verified else state==unsafe
+    ensures expiry_time==old(expiry_time)
     {
         if safe(curr_time) && accepted {
             state:=verified;
+			success:=true;
         } else {
             state:=unsafe;
+			success:=false;
         }
 
         blood_type:=determined_type;
         rhesus:=rhesus_in;
     }
 
-    method store_blood(curr_time:int)
+    method store_blood(curr_time:int) returns (success:bool)
     modifies this
     requires Valid()
     requires state==verified;
     ensures if safe(curr_time) then state == storage else state==unsafe;
     ensures Valid()
+	ensures if success then state==storage else state==unsafe
+	ensures safe(curr_time) == success
+	ensures blood_type==old(blood_type)
+	ensures rhesus == old(rhesus)
+    ensures expiry_time==old(expiry_time)
     {
         if safe(curr_time) {
             state:=storage;
+			success:=true;
         } else {
             state:=unsafe;
+			success:=false;
         }  
     }
 
-    method dispatch_blood(curr_time:int)
+    method dispatch_blood(curr_time:int) returns (success:bool)
     modifies this
     requires Valid()
     requires state==storage;
     ensures if safe(curr_time) then state == dispatched else state==unsafe;
     ensures Valid()
+	ensures if success then state==dispatched else state==unsafe
+	ensures blood_type==old(blood_type)
+	ensures rhesus == old(rhesus)
+    ensures expiry_time==old(expiry_time)
     {
         if safe(curr_time) {
             state:=dispatched;
+			success:=true;
         } else {
             state:=unsafe;
-        }         
+			success:=false;
+        }
     }
 
-    method deliver_blood(curr_time:int)
+    method deliver_blood(curr_time:int) returns (success:bool)
     modifies this
     requires Valid()
     requires state==dispatched;
     ensures if safe(curr_time) then state ==delivered else state==unsafe;
     ensures Valid()
+	ensures if success then state==delivered else state==unsafe
+	ensures blood_type==old(blood_type)
+	ensures rhesus == old(rhesus)
+    ensures expiry_time==old(expiry_time)
     {
         if safe(curr_time) {
             state:=delivered;
+			success:=true;
         } else {
             state:=unsafe;
+			success:=false;
         }           
     }
 
@@ -138,142 +161,3 @@ class Blood{
     ensures Valid()
     {state:=unsafe;}
 }
-
-//#include blood.dfy
-
-class transportationManager {
-	
-	var locale: int; // give each location an int value?
-	var destinations: array<int>; //:= new int[10]; // routes to destinations
-	var toSend: array<Blood>;// := new Blood[10]; // may need to have another array that matches the blood destinations to each index or create a class that can hold blood and its dest
-    	var toDest: array<int>;// := new int[10]; // routes (match with toSend array)
-
-    	
-
-	// Blood always has a destination, ie every blood in array is matched by a route
-	predicate method Valid()
-	//requires toDest != null;
-	//requires toSend != null
-	reads this;
-	//reads toDest[0],toDest[1], toDest[2],toDest[3],toDest[4],toDest[5],toDest[6],toDest[7],toDest[8],toDest[9];
-	requires toDest != null;
-	requires toSend != null;
-	{
-        	//forall x,y:: 0 <= x < toDest.Length && 0 <= y < toSend.Length && x == y ==> toDest[x]!=-1 && toSend[y] != null
-    		toDest !=null && toSend != null
-	}
-
-
-	method Init(src: int)
-	modifies this;
-	modifies toDest;
-	modifies toSend;
-	modifies `locale;
-	requires src >= 0
-	ensures toDest != null;
-	ensures toSend != null;
-	ensures Valid()
-	{
-		locale := src;
-		toDest := new int[10];
-		toSend := new Blood[10];
-		//var i := 0;
-		//assert toSend != null;
-		//while (i < toSend.Length) 
-		//invariant 0 <= i < toSend.Length
-		//{	
-		//	toSend[i] := null;
-		//	i := i + 1;
-		//}
-		//i := 0;
-		//while (i < toDest.Length)
-		//invariant 0 <= i < toDest.Length
-		//{
-		//	toDest[i] := -1;
-		//	i := i + 1;
-		//}
-	}
-
-		
-	method receive(bld:Blood, dst:int)
-	modifies this.toDest
-	modifies this.toSend 
-	requires toSend != null
-	requires toDest != null
-	requires forall x :: 0 <= x < toSend.Length ==> bld != toSend[x] // blood is not already in toSend
-	requires bld != null;
-	requires toSend.Length == toDest.Length
-	requires dst >= 0;
-	requires Valid(); ensures Valid();
-	//ensures forall x, y:: 0 <= x < toSend.Length && 0 <= y < toDest.Length && x == y ==> toSend[x] == bld && toDest[y] == dst -> need to fix
-	{
-       		var cDest := -1;
-		if (dst == -1) {
-			cDest := 3; // need to grab the dest that system spits out
-		} else {
-			cDest := -1;
-		}
-		//var index := 0;
-		//var i := 0;
-		//while (index < toSend.Length) 
-		//invariant 0 <= i <= toSend.Length
-		//{
-		//	if (toSend[i] == null) {
-		//		index := i;
-		//		i := toSend.Length -1;		
-		//	}
-		//	i :=  i + 1;
-		//}
-		//toSend[i] := bld;
-		//toDest[i] := cDest;
-
-		var i := 0;
-		var j := 0;
-		while (i < toSend.Length && j < toDest.Length)
-		invariant 0 <= i <= toSend.Length
-		invariant 0 <= j <= toDest.Length
-		//invariant forall x,y :: 0 <= x < toSend.Length && 0 <= y < toDest.Length && toDest[y] == cDest && toSend[x] == bld ==> (x==y) -> need to fix
-		//invariant forall x :: 0 <= x < (j-1) ==> toDest[x] != 0
-		//invariant forall x, y :: 0 <= x < i && 0 <= y < j && x == y ==> toSend[x] == bl
-		invariant i == j
-		{
-			if (toSend[i] == null && toDest[j] == 0) {
-				toSend[i] := bld;
-				toDest[j] := cDest;
-				//i := toSend.Length -1;
-				//j := toDest.Length -1;
-			}
-			i := i + 1;
-			j := j + 1;
-		}
-    	}
-
-
-	method dispatchBlood()
-	modifies toSend;
-	modifies toDest;
-	requires toSend != null;
-	requires toDest != null;
-	requires exists x :: 0 <= x < toSend.Length && toSend[x] != null // blood is to be sent
-	requires Valid();ensures Valid();
-    	ensures forall x, y:: 0 <= x < toSend.Length && 0 <= y < toDest.Length  && x == y ==> (toSend[x] == null && toDest[y] == 0) // toSend and toRoute are empty
-	{
-		var i := 0;
-		var j := 0;
-		while (i < toSend.Length && j < toDest.Length)
-		invariant 0 <= i <= toSend.Length
-		invariant 0 <= j <= toDest.Length
-		invariant forall x :: 0 <= x < i ==> toSend[x] == null
-		invariant forall x :: 0 <= x < j ==> toDest[x] == 0
-		invariant i == j
-		{
-			toDest[j] := 0;
-			toSend[i] := null;
-			i := i + 1;
-			j := j + 1;
-		}
-		
-    	}
-    
-}
-
